+-comm : ∀ (m n : ℕ) → m + n ≡ n + m
+-comm m zero =
  begin
    m + zero
  ≡⟨ +-identityʳ m ⟩
    m
  ≡⟨⟩
    zero + m
  ∎
+-comm m (suc n) =
  begin
    m + suc n
  ≡⟨ +-suc m n ⟩
    suc (m + n)
  ≡⟨ cong suc (+-comm m n) ⟩
    suc (n + m)
  ≡⟨⟩
    suc n + m
  ∎

+-assoc : ∀ (m n p : ℕ) → (m + n) + p ≡ m + (n + p)
+-assoc zero n p =
  begin
    (zero + n) + p
  ≡⟨⟩
    n + p
  ≡⟨⟩
   zero + (n + p)
  ∎
+-assoc (suc m) n p =
  begin
    (suc m + n) + p
  ≡⟨⟩
    suc (m + n) + p
  ≡⟨⟩
    suc ((m + n) + p)
  ≡⟨ cong suc (+-assoc m n p) ⟩
    suc (m + (n + p))
  ≡⟨⟩
    suc m + (n + p)
  ∎


+-swap : ∀ (m n p : ℕ) → m + (n + p) ≡ n + (m + p)
+-swap zero n p =
  begin
    zero + (n + p)
  ≡⟨⟩
    n + p
  ≡⟨⟩
    n + (zero + p)
  ∎
+-swap (suc m) n p =
  begin
    suc m + (n + p)
  ≡⟨ cong suc (+-assoc m n p) ⟩
    suc (m + n) + p
  ≡⟨⟩
    suc ((m + n) + p)
  ≡⟨ cong suc (+-comm m n) ⟩
    suc ((n + m) + p)
  ≡⟨⟩
    suc n + (m + p)
  ∎
